Bonak/νSet.lean
@@ -146,5 +146,101 @@ def mkRestrPaintingTypes (A : AritySig) :
           (A := A) (DepsRestrExtension.AddRestrDep extraDeps) &T
         mkRestrPaintingType A extraDeps }
 
+structure CohFrameTypeBlock (A : AritySig) {p k : Nat}
+    (extraDeps : DepsRestrExtension A p k) where
+  CohFrameTypesDef : Type 1
+  RestrFramesDef : CohFrameTypesDef -> mkRestrFrameTypes A (mkPaintings A extraDeps)
+
+def mkCohFrameTypesStep (A : AritySig) {p k : Nat}
+    (extraDeps : DepsRestrExtension A p.succ k)
+    (prev : CohFrameTypeBlock A (DepsRestrExtension.AddRestrDep extraDeps)) :
+    Type 1 :=
+  { Q : prev.CohFrameTypesDef &T
+    forall (q : Nat) (Hq : leR q k) (r : Nat) (Hr : leR r q)
+      (eps omega : A.arity)
+      (d : mkFrame A (proj1DepsRestr A (toDepsRestr A (prev.RestrFramesDef Q)))),
+      extraDeps.deps.restrFrames.2 q Hq eps
+        ((prev.RestrFramesDef Q).2 r (leR_trans Hr (leR_up Hq)) omega d) =
+      extraDeps.deps.restrFrames.2 r (leR_trans Hr Hq) omega
+        ((prev.RestrFramesDef Q).2 q.succ (leR_raise_both Hq) eps d) }
+
+def mkRestrLayer (A : AritySig) {p k : Nat}
+    {extraDeps : DepsRestrExtension A p.succ k}
+    (restrPaintings : mkRestrPaintingTypes A extraDeps)
+    {prev : CohFrameTypeBlock A (DepsRestrExtension.AddRestrDep extraDeps)}
+    (cohFrames : mkCohFrameTypesStep A extraDeps prev)
+    (q : Nat) (Hq : leR q k) (eps : A.arity)
+    (d : mkFrame A (proj1DepsRestr A (toDepsRestr A (prev.RestrFramesDef cohFrames.1)))) :
+    mkLayer A (mkPaintings A (DepsRestrExtension.AddRestrDep extraDeps))
+      (prev.RestrFramesDef cohFrames.1) d ->
+    mkLayer A extraDeps.deps.paintings extraDeps.deps.restrFrames
+      ((prev.RestrFramesDef cohFrames.1).2 q.succ (leR_raise_both Hq) eps d) :=
+  fun l omega =>
+    transport (fun x => (extraDeps.deps.paintings.2 x).Dom)
+      (cohFrames.2 q Hq 0 leR_O eps omega d)
+      (restrPaintings.2 q Hq eps _ (l omega))
+
+def mkCohFrameTypesAndRestrFrames (A : AritySig) :
+    {p k : Nat} -> (extraDeps : DepsRestrExtension A p k) ->
+      mkRestrPaintingTypes A extraDeps -> CohFrameTypeBlock A extraDeps
+  | 0, _, _, _ =>
+      { CohFrameTypesDef := PUnit.{2}
+        RestrFramesDef := fun _ => (PUnit.unit ; fun _ _ _ _ => PUnit.unit) }
+  | _ + 1, _, extraDeps, restrPaintings =>
+      let prev := mkCohFrameTypesAndRestrFrames A
+        (DepsRestrExtension.AddRestrDep extraDeps) restrPaintings.1
+      let restrFrames := prev.RestrFramesDef
+      { CohFrameTypesDef := mkCohFrameTypesStep A extraDeps prev
+        RestrFramesDef := fun Q =>
+          (restrFrames Q.1 ;
+            fun q Hq eps d =>
+              ((restrFrames Q.1).2 q.succ (leR_raise_both Hq) eps d.1 ;
+                mkRestrLayer A restrPaintings Q q Hq eps d.1 d.2)) }
+
+abbrev mkCohFrameTypes (A : AritySig) {p k : Nat}
+    {extraDeps : DepsRestrExtension A p k}
+    (restrPaintings : mkRestrPaintingTypes A extraDeps) : Type 1 :=
+  (mkCohFrameTypesAndRestrFrames A extraDeps restrPaintings).CohFrameTypesDef
+
+structure DepsCohs (A : AritySig) (p k : Nat) where
+  extraDeps : DepsRestrExtension A p k
+  restrPaintings : mkRestrPaintingTypes A extraDeps
+  cohs : mkCohFrameTypes A restrPaintings
+
+abbrev DepsCohs.deps {A : AritySig} {p k : Nat}
+    (depsCohs : DepsCohs A p k) : DepsRestr A p k :=
+  depsCohs.extraDeps.deps
+
+def toDepsCohs (A : AritySig) {p k : Nat}
+    {extraDeps : DepsRestrExtension A p k}
+    {restrPaintings : mkRestrPaintingTypes A extraDeps}
+    (cohs : mkCohFrameTypes A restrPaintings) : DepsCohs A p k :=
+  { extraDeps := extraDeps
+    restrPaintings := restrPaintings
+    cohs := cohs }
+
+def proj1DepsCohs (A : AritySig) {p k : Nat}
+    (depsCohs : DepsCohs A p.succ k) : DepsCohs A p k.succ :=
+  { extraDeps := DepsRestrExtension.AddRestrDep depsCohs.extraDeps
+    restrPaintings := depsCohs.restrPaintings.1
+    cohs := depsCohs.cohs.1 }
+
+abbrev mkRestrFrames (A : AritySig) {p k : Nat}
+    (depsCohs : DepsCohs A p k) :
+    mkRestrFrameTypes A (mkPaintings A depsCohs.extraDeps) :=
+  (mkCohFrameTypesAndRestrFrames A depsCohs.extraDeps
+    depsCohs.restrPaintings).RestrFramesDef depsCohs.cohs
+
+def mkDepsRestr (A : AritySig) {p k : Nat}
+    (depsCohs : DepsCohs A p k) : DepsRestr A p.succ k :=
+  toDepsRestr A (mkRestrFrames A depsCohs)
+
+abbrev mkRestrFrame (A : AritySig) {p k : Nat}
+    (depsCohs : DepsCohs A p k) :
+    forall q : Nat, leR q k -> A.arity ->
+      mkFrame A (proj1DepsRestr A (mkDepsRestr A depsCohs)) ->
+      mkFrame A depsCohs.deps :=
+  (mkRestrFrames A depsCohs).2
+
 end νSet
 end Bonak
